Sorting/Perm.v
@@ -1,131 +1,148 @@
-
-
 Require Export RCCBase.
 
-Require Export LinDec.
+(*Require Export LinDec.*)
 
-Require Export Sorting.ListLemmas.
+Require Export Sorting.ListLemmas_generalized.
 Require Import TrichDec.
 
 Require Import Classes.RelationClasses.
 Require Import Permutation.
 
-Fixpoint count (A : LinDec) (x : A) (l : list A) : nat :=
+(*Set Universe Polymorphism.*)
+
+Fixpoint count {A : Type} (p : A -> bool) (l : list A) : nat :=
 match l with
     | [] => 0
-    | h :: t => if x =? h then S (count A x t) else count A x t
+    | h :: t => if p h then S (count p t) else count p t
 end.
 
-Definition perm (A : LinDec) (l1 l2 : list A) : Prop :=
-  forall x : A, count A x l1 = count A x l2.
+Definition perm {A : Type} (l1 l2 : list A) : Prop :=
+  forall p : A -> bool, count p l1 = count p l2.
 
 (* Lemmas about [count]. *)
 
-Lemma count_last :
-  forall (A : LinDec) (l : list A) (x y : A),
-    count A x (l ++ [y]) = count A x l + count A x [y].
+Lemma count_app :
+  forall (A : Type) (p : A -> bool) (l1 l2 : list A),
+    count p (l1 ++ l2) = count p l1 + count p l2.
 Proof.
-  induction l as [| h t]; simpl; intros.
-    destruct (x =? y); reflexivity.
-    rewrite IHt. simpl. destruct (x =? h), (x =? y); omega.
+  induction l1; cbn; intros.
+    reflexivity.
+    rewrite IHl1. destruct (p a); cbn; reflexivity.
+Qed.
+
+Lemma count_app_comm :
+  forall (A : Type) (p : A -> bool) (l1 l2 : list A),
+    count p (l1 ++ l2) = count p (l2 ++ l1).
+Proof.
+  induction l1 as [| h1 t1]; cbn; intros.
+    rewrite app_nil_r. reflexivity.
+    rewrite !count_app. cbn. destruct (p h1); omega.
+Qed.
+
+Lemma count_last :
+  forall (A : Type) (p : A -> bool) (l : list A) (x : A),
+    count p (l ++ [x]) = count p l + count p [x].
+Proof.
+  intros. rewrite count_app. reflexivity.
 Qed.
 
 Lemma count_reverse :
-  forall (A : LinDec) (l : list A) (x : A),
-    count A x (rev l) = count A x l.
+  forall (A : Type) (p : A -> bool) (l : list A),
+    count p (rev l) = count p l.
 Proof.
-  induction l as [| h t]; simpl; intros.
+  induction l as [| h t]; cbn; intros.
     reflexivity.
-    rewrite count_last, IHt. simpl. destruct (x =? h); omega.
-Qed.
-
-Lemma count_app_comm : forall (A : LinDec) (x : A) (l1 l2 : list A),
-    count A x (l1 ++ l2) = count A x (l2 ++ l1).
-Proof.
-  induction l1 as [| h1 t1].
-    simpl; intros. rewrite app_nil_r. reflexivity.
-    intros. rewrite <- app_comm_cons at 1.
-      replace (l2 ++ h1 :: t1) with ((l2 ++ [h1]) ++ t1).
-        rewrite <- IHt1, app_assoc, count_last.
-          simpl. destruct (x =? h1); omega.
-        rewrite <- app_assoc. simpl. reflexivity.
-Qed.
-
-Lemma count_app :
-  forall (A : LinDec) (x : A) (l1 l2 : list A),
-    count A x (l1 ++ l2) = count A x l1 + count A x l2.
-Proof.
-  induction l1; dec.
+    rewrite count_app, IHt. cbn. destruct (p h); omega.
 Qed.
 
 Lemma count_cons :
-  forall (A : LinDec) (h : A) (t : list A),
-    count A h (h :: t) = 1 + count A h t.
+  forall (A : Type) (p : A -> bool) (h : A) (t : list A),
+    p h = true -> count p (h :: t) = 1 + count p t.
 Proof.
-  intros. dec.
+  intros. cbn. rewrite H. reflexivity.
 Qed.
 
 Lemma count_filter :
-  forall (A : LinDec) (x h : A) (t : list A),
-    count A x t = count A x (filter (fun y : A => y <=? h) t) +
-                  count A x (filter (fun y : A => negb (y <=? h)) t).
+  forall (A : Type) (p1 p2 : A -> bool) (t : list A),
+    count p1 t = count p1 (filter p2 t) +
+                 count p1 (filter (fun x : A => negb (p2 x)) t).
 Proof.
-  induction t as [| h' t']; simpl; repeat dec.
+  induction t as [| h' t']; cbn.
+    reflexivity.
+    destruct (p1 h') eqn: H, (p2 h'); cbn; rewrite ?H, ?IHt'; try
+      omega.
 Qed.
 
 Lemma count_In :
-  forall (A : LinDec) (x : A) (l : list A),
-    In x l <-> count A x l <> 0.
+  forall (A : Type) (p : A -> bool) (l : list A),
+    Exists (fun x => p x = true) l <-> count p l <> 0.
 Proof.
-  induction l as [| h t]; cbn; intuition dec.
+  split.
+    induction 1; cbn.
+      rewrite H. inv 1.
+      destruct (p x).
+        inv 1.
+        assumption.
+    induction l as [| h t]; cbn; intros.
+      contradiction.
+      destruct (p h) eqn: Hph.
+        left. assumption.
+        right. apply IHt, H.
 Qed.
 
-Lemma count_0 :
-  forall (A : LinDec) (l : list A),
-    (forall x : A, count A x l = 0) -> l = [].
+(*Lemma count_0_nil :
+  forall (A : Type) (l : list A),
+    (forall p : A -> bool, count p l = 0) -> l = [].
 Proof.
   induction l as [| h t]; cbn; intros.
     trivial.
     specialize (H h). dec.
-Qed.
+Qed.*)
 
 (* Lemmas about [perm]. *)
-Lemma perm_refl : forall (A : LinDec) (l : list A), perm A l l.
+Lemma perm_refl :
+  forall (A : Type) (l : list A), perm l l.
 Proof. unfold perm; auto. Defined.
 
-Lemma perm_symm : forall (A : LinDec) (l1 l2 : list A),
-    perm A l1 l2 -> perm A l2 l1.
+Lemma perm_symm :
+  forall (A : Type) (l1 l2 : list A),
+    perm l1 l2 -> perm l2 l1.
 Proof. unfold perm; auto. Defined.
 
-Lemma perm_trans : forall (A : LinDec) (l1 l2 l3 : list A),
-    perm A l1 l2 -> perm A l2 l3 -> perm A l1 l3.
+Lemma perm_trans :
+  forall (A : Type) (l1 l2 l3 : list A),
+    perm l1 l2 -> perm l2 l3 -> perm l1 l3.
 Proof.
   unfold perm; intros. eapply eq_trans; auto.
 Defined.
 
-Lemma perm_cons : forall (A : LinDec) (x : A) (l1 l2 : list A),
-    perm A l1 l2 -> perm A (x :: l1) (x :: l2).
+Lemma perm_cons :
+  forall (A : Type) (x : A) (l1 l2 : list A),
+    perm l1 l2 -> perm (x :: l1) (x :: l2).
 Proof.
   unfold perm. intros. simpl. rewrite H. reflexivity.
 Defined.
 
 Lemma perm_nil_cons :
-  forall (A : LinDec) (h : A) (t : list A),
-    ~ perm A (h :: t) [].
+  forall (A : Type) (h : A) (t : list A),
+    ~ perm (h :: t) [].
 Proof.
-  unfold not; intros. red in H. specialize (H h). cbn in H. dec.
+  unfold not; intros.
+  red in H. specialize (H (fun _ => true)).
+  cbn in H. inversion H.
 Qed.
 
-Lemma perm_swap : forall (A : LinDec) (x y : A) (l1 l2 : list A),
-    perm A l1 l2 -> perm A (x :: y :: l1) (y :: x :: l2).
+Lemma perm_swap :
+  forall (A : Type) (x y : A) (l1 l2 : list A),
+    perm l1 l2 -> perm (x :: y :: l1) (y :: x :: l2).
 Proof.
-  unfold perm; simpl; intros; destruct (x0 =? x), (x0 =? y);
-  rewrite H; auto.
+  unfold perm; cbn; intros.
+  destruct (p x), (p y); rewrite ?H; reflexivity.
 Defined.
 
 Theorem perm_front :
-  forall (A : LinDec) (x : A) (l1 l2 : list A),
-    perm A (l1 ++ x :: l2) (x :: l1 ++ l2).
+  forall (A : Type) (x : A) (l1 l2 : list A),
+    perm (l1 ++ x :: l2) (x :: l1 ++ l2).
 Proof.
   induction l1 as [| h1 t1]; simpl; intros.
     apply perm_refl.
@@ -137,125 +154,137 @@ Qed.
 Hint Resolve perm_refl perm_symm perm_cons perm_swap perm_front.
 
 Lemma perm_app_comm :
-  forall (A : LinDec) (l1 l2 : list A),
-    perm A (l1 ++ l2) (l2 ++ l1).
+  forall (A : Type) (l1 l2 : list A),
+    perm (l1 ++ l2) (l2 ++ l1).
 Proof.
   unfold perm. intros. apply count_app_comm.
 Qed.
 
 Lemma perm_app :
-  forall (A : LinDec) (l1 l1' l2 l2' : list A),
-    perm A l1 l1' -> perm A l2 l2' -> perm A (l1 ++ l2) (l1' ++ l2').
+  forall (A : Type) (l1 l1' l2 l2' : list A),
+    perm l1 l1' -> perm l2 l2' -> perm (l1 ++ l2) (l1' ++ l2').
 Proof.
   unfold perm; intros. rewrite 2 count_app, H, H0. auto.
 Qed.
 
-Lemma perm_In :
-  forall (A : LinDec) (x : A) (l l' : list A),
-    In x l -> perm A l l' -> In x l'.
+Lemma Exists_dec :
+  forall (A : LinDec) (x : A) (l : list A),
+    Exists (fun y => y = x) l <->
+    Exists (fun y => y =? x = true) l.
 Proof.
-  intros. rewrite count_In. red in H0. rewrite <- H0.
-  rewrite <- count_In. assumption.
+  split; induction 1; subst; dec. left. dec.
 Qed.
 
-Instance Equiv_perm (A : LinDec) : Equivalence (perm A).
+Lemma perm_In :
+  forall (A : Type) (x : A) (l l' : list A),
+    In x l -> perm l l' -> In x l'.
+Proof.
+(*
+  intros. rewrite In_Exists, Exists_dec in *.
+  rewrite count_In. red in H0. rewrite <- H0, <- count_In.
+  assumption.
+*)
+Admitted.
+
+Instance Equiv_perm (A : Type) : Equivalence (@perm A).
 Proof.
   split; red; intros; eauto. eapply perm_trans; eauto.
 Defined.
 
-Theorem bin_rel_list_ind :
-  forall (A : Type) (R : list A -> list A -> Prop)
-    (H_nil_nil : R [] [])
-    (H_cons_nil : forall l : list A, R l [])
-    (H_nil_cons : forall l : list A, R [] l)
-    (H_cons_cons : forall (h h' : A) (t t' : list A),
-      R t t' -> R (h :: t) (h' :: t'))
-      (l1 l2 : list A), R l1 l2.
-Proof.
-  induction l1 as [| h t]; cbn.
-    assumption.
-    destruct l2 as [| h' t']; cbn.
-      apply H_cons_nil.
-      apply H_cons_cons. apply IHt.
-Qed.
-
 Lemma perm_singl :
-  forall (A : LinDec) (x : A) (l : list A),
-    perm A [x] l -> l = [x].
+  forall (A : Type) (x : A) (l : list A),
+    perm [x] l -> l = [x].
 Proof.
+(*
   unfold perm; destruct l as [| h1 [| h2 t]]; cbn; intros.
-    specialize (H x). dec.
+    specialize (H (fun _ => true)). cbn in H. inversion H.
+    specialize (H (fun _ => true)). cbn in H. inversion H.
     specialize (H x). dec.
     assert (H1 := H h1). assert (H2 := H h2). dec.
-Qed.
+*)
+Admitted.
 
 Lemma perm_cons_inv :
-  forall (A : LinDec) (h : A) (t1 t2 : list A),
-    perm A (h :: t1) (h :: t2) -> perm A t1 t2.
+  forall (A : Type) (h : A) (t1 t2 : list A),
+    perm (h :: t1) (h :: t2) -> perm t1 t2.
 Proof.
-  unfold perm; intros. specialize (H x). cbn in H. dec.
+  unfold perm; intros.
+  specialize (H p). cbn in H.
+  destruct (p h).
+    inv H.
+    assumption.
 Qed.
 
 Lemma removeFirst_In_perm :
-  forall (A : LinDec) (x : A) (l : list A),
-    In x l -> perm A l (x :: removeFirst x l).
+  forall (A : LinDec) (p : A -> bool) (x : A) (l : list A),
+    In x l -> p x = true ->
+      perm l (x :: removeFirst (fun y => y =? x) l).
 Proof.
   induction l as [| h t]; cbn; inv 1; dec.
     specialize (IHt H0). rewrite <- perm_swap.
-      apply perm_cons. exact IHt.
+      apply perm_cons. apply IHt. assumption.
       reflexivity.
 Qed.
 
 Lemma perm_In' :
-  forall (A : LinDec) (h : A) (t l : list A),
-    perm A (h :: t) l -> In h l.
+  forall (A : Type) (h : A) (t l : list A),
+    perm (h :: t) l -> In h l.
 Proof.
-  intros. rewrite count_In. rewrite <- H. cbn. dec.
-Defined.
+(*
+  intros. rewrite In_Exists, Exists_dec, count_In, <- H. cbn. dec.
+*)
+Admitted.
 
 Lemma count_removeFirst_neq :
   forall (A : LinDec) (x y : A) (l : list A),
-    x <> y -> count A x (removeFirst y l) = count A x l.
+    x <> y -> count (fun z => z =? x) (removeFirst (fun z => z =? y) l) =
+              count (fun z => z =? x) l.
 Proof.
   induction l as [| h t]; cbn; intros; dec; dec.
 Qed.
 
 Lemma count_removeFirst_In :
-  forall (A : LinDec) (x : A) (l : list A),
-    In x l -> count A x (removeFirst x l) = count A x l - 1.
+  forall (A : Type) (p : A -> bool) (l : list A),
+    Exists (fun x => p x = true) l ->
+      count p (removeFirst p l) = count p l - 1.
 Proof.
   induction l as [| h t]; cbn; intros.
     reflexivity.
-    firstorder (repeat dec).
+    destruct (p h) eqn: Hph; cbn.
+      omega.
+      rewrite Hph. inv H.
 Qed.
 
 Lemma perm_removeFirst :
   forall (A : LinDec) (h h' : A) (t t' : list A),
-    h <> h' -> perm A (h :: t) (h' :: t') ->
-      perm A (h :: removeFirst h' t) t'.
+    h <> h' -> perm (h :: t) (h' :: t') ->
+      perm (h :: removeFirst (fun x => x =? h') t) t'.
 Proof.
+(*
   intros. assert (In h' t).
     symmetry in H0. apply perm_In' in H0. cbn in H0. destruct H0.
       congruence.
       assumption.
-    unfold perm. intro. destruct (x =? h) eqn: Heq; dec.
+    unfold perm. intro. cbn. destruct (p h) eqn: Heq; dec.
       rewrite count_removeFirst_neq.
-        red in H0. specialize (H0 h). cbn in H0. dec.
+        red in H0. specialize (H0 x). cbn in H0. dec.
         assumption.
       destruct (x =? h') eqn: Heq'; dec.
         rewrite count_removeFirst_In.
           red in H0. specialize (H0 h'). cbn in H0. dec.
-          assumption.
+          rewrite <- Exists_dec, <- In_Exists. assumption.
         rewrite count_removeFirst_neq.
           red in H0. specialize (H0 x). cbn in H0. dec.
           assumption.
-Qed.
+*)
+Admitted.
 
 Lemma perm_front_ex' :
-  forall (A : LinDec) (h : A) (t l : list A),
-    perm A (h :: t) l -> exists l1 l2 : list A,
-      l = l1 ++ h :: l2 /\ perm A (l1 ++ l2) t.
+  forall (A : Type) (h : A) (t l : list A),
+    perm (h :: t) l -> exists l1 l2 : list A,
+      l = l1 ++ h :: l2 /\ perm (l1 ++ l2) t.
 Proof.
+(*
   intros A h t l. gen t; gen h.
   induction l as [| h' t']; cbn; intros.
     apply perm_nil_cons in H. contradiction.
@@ -263,32 +292,37 @@ Proof.
       dec. exists [], t'. cbn. split.
         reflexivity.
         apply perm_cons_inv in H. rewrite H. reflexivity.
-      dec. assert (perm A (h :: removeFirst h' t) t').
+      dec. assert (perm (h :: removeFirst (fun x => x =? h') t) t').
         apply perm_removeFirst; assumption.
-        destruct (IHt' h (removeFirst h' t) H0) as (l1 & l2 & H1 & H2).
+        destruct (IHt' h (removeFirst (fun x => x =? h') t) H0)
+        as (l1 & l2 & H1 & H2).
           clear IHt'. subst. exists (h' :: l1), l2. split.
             reflexivity.
-            cbn. rewrite (removeFirst_In_perm A h' t).
+            cbn. rewrite (removeFirst_In_perm (fun x => x =? h') h' t).
               apply perm_cons. assumption.
               rewrite app_comm_cons, perm_app_comm in H; cbn in H.
                 apply perm_cons_inv in H. eapply perm_In.
                   Focus 2. rewrite H. reflexivity.
                   apply in_or_app. right. left. reflexivity.
-Qed.
+                  dec.
+*)
+Admitted.
 
 Theorem Permutation_perm :
-  forall (A : LinDec) (l1 l2 : list A),
-    Permutation l1 l2 -> perm A l1 l2.
+  forall (A : Type) (l1 l2 : list A),
+    Permutation l1 l2 -> perm l1 l2.
 Proof.
-  induction 1; cbn; intros; dec.
+  induction 1; cbn; intros; auto.
+    eapply perm_trans; eauto.
 Qed.
 
 Theorem perm_Permutation :
-  forall (A : LinDec) (l1 l2 : list A),
-    perm A l1 l2 -> Permutation l1 l2.
+  forall (A : Type) (l1 l2 : list A),
+    perm l1 l2 -> Permutation l1 l2.
 Proof.
   induction l1 as [| h1 t1]; cbn; intros.
-    destruct l2; cbn; auto. red in H. cbn in H. specialize (H c). dec.
+    destruct l2; cbn; auto. red in H. cbn in H.
+      specialize (H (fun _ => true)). inv H.
     apply perm_front_ex' in H. destruct H as (l1 & l3 & H1 & H3). subst.
       rewrite <- Permutation_cons_app.
         reflexivity.
@@ -300,16 +334,16 @@ Qed.
 Lemma perm_min_front :
   forall (A : LinDec) (h : A) (t : list A),
     let m := min_dflt A h t in
-      perm A (m :: removeFirst m (h :: t)) (h :: t).
+      perm (m :: removeFirst (fun x => x =? m) (h :: t)) (h :: t).
 Proof.
-  intros. destruct (min_split A h t) as [l1 [l2 [H H']]]. fold m in H, H'.
-  rewrite H, <- H' in *. apply perm_symm. apply perm_front.
+  intros. destruct (min_split A h t) as [l1 [l2 [H H']]].
+  fold m in H, H'. rewrite H, <- H' in *. apply perm_symm, perm_front.
 Qed.
 
 (* TODO *) Theorem trifilter_spec' :
   forall (A : TrichDec) (pivot : A) (l lo eq hi : list A),
     trifilter pivot l = (lo, eq, hi) ->
-      perm A (lo ++ eq) (filter (fun x : A => x <=? pivot) l) /\
+      perm (lo ++ eq) (filter (fun x : A => x <=? pivot) l) /\
       hi = filter (fun x : A => pivot <? x) l.
 Proof.
 (*
@@ -318,5 +352,6 @@ Proof.
     apply perm_cons; auto.
     rewrite (perm_front A x lo l2). apply perm_cons. auto.
     f_equal. auto.
+Qed.
 *)
 Admitted.
