Sorting/Sort.v
@@ -1,24 +1,20 @@
-
-
 Require Export RCCBase.
 
 Require Export Sorting.Perm.
 
-Inductive Sorted (A : LinDec) : list A -> Prop :=
-    | Sorted0 : Sorted A []
-    | Sorted1 : forall x : A, Sorted A [x]
+Inductive Sorted {A : Type} (R : A -> A -> Prop) : list A -> Prop :=
+    | Sorted0 : Sorted R []
+    | Sorted1 : forall x : A, Sorted R [x]
     | Sorted2 : forall (x y : A) (l : list A),
-        x ≤ y -> Sorted A (y :: l) -> Sorted A (x :: y :: l).
+        R x y -> Sorted R (y :: l) -> Sorted R (x :: y :: l).
 
 Hint Constructors Sorted.
 
-Class Sort (A : LinDec) : Type :=
+Class Sort {A : Type} (R : A -> A -> Prop) : Type :=
 {
     sort :> list A -> list A;
     Sorted_sort :
-      forall l : list A, Sorted A (sort l);
-(*    sort_perm :
-      forall l : list A, perm A l (sort l);*)
+      forall l : list A, Sorted R (sort l);
     Permutation_sort :
       forall l : list A, Permutation (sort l) l
 }.
@@ -26,33 +22,70 @@ Class Sort (A : LinDec) : Type :=
 Coercion sort : Sort >-> Funclass.
 
 Lemma sort_perm :
-  forall (A : LinDec) (s : Sort A) (l : list A),
-    perm A l (sort l).
+  forall (A : Type) (R : A -> A -> Prop) (s : Sort R) (l : list A),
+    perm l (sort l).
 Proof.
   intros. apply Permutation_perm. rewrite Permutation_sort. reflexivity.
 Qed.
 
+(*
+Class Partition (A : Type) (R : A -> A -> Prop) : Type :=
+{
+    partition :> A -> list A -> list A * list A * list A;
+    spec_lo :
+      forall (pivot : A) (l lo eq hi : list A),
+        partition pivot l = (lo, eq, hi) ->
+          forall x : A, In x lo -> R x pivot;
+    spec_eq :
+      forall (pivot : A) (l lo eq hi : list A),
+        partition pivot l = (lo, eq, hi) ->
+          forall x : A, In x eq -> x = pivot;
+    spec_hi :
+      forall (pivot : A) (l lo eq hi : list A),
+        partition pivot l = (lo, eq, hi) ->
+          forall x : A, In x hi -> R pivot x /\ pivot <> x;
+    len_lo :
+      forall (pivot : A) (l lo eq hi : list A),
+        partition pivot l = (lo, eq, hi) ->
+          length lo <= length l;
+    len_eq :
+      forall (pivot : A) (l lo eq hi : list A),
+        partition pivot l = (lo, eq, hi) ->
+          length eq <= length l;
+    len_hi :
+      forall (pivot : A) (l lo eq hi : list A),
+        partition pivot l = (lo, eq, hi) ->
+          length hi <= length l;
+    partition_perm :
+      forall (pivot : A) (l lo eq hi : list A),
+        partition pivot l = (lo, eq, hi) ->
+          Permutation l (lo ++ eq ++ hi);
+}.
+
+Coercion partition : Partition >-> Funclass.
+*)
+
 (* Lemmas about [Sorted]. *)
 
 Theorem Sorted_tail :
-  forall (A : LinDec) (h : A) (t : list A),
-    Sorted A (h :: t) -> Sorted A t.
+  forall (A : Type) (R : A -> A -> Prop) (h : A) (t : list A),
+    Sorted R (h :: t) -> Sorted R t.
 Proof.
   inversion 1; auto.
 Defined.
 
 Theorem Sorted_head :
-  forall (A : LinDec) (x y : A) (l : list A),
-    Sorted A (x :: y :: l) -> x ≤ y.
+  forall (A : Type) (R : A -> A -> Prop) (x y : A) (l : list A),
+    Sorted R (x :: y :: l) -> R x y.
 Proof.
   inversion 1. assumption.
 Qed.
 
 Lemma Sorted_app_all :
-  forall (A : LinDec) (l : list A) (h : A) (t : list A),
-    Sorted A l -> Sorted A (h :: t) ->
-    (forall x : A, In x l -> leq x h) ->
-      Sorted A (l ++ h :: t).
+  forall (A : Type) (R : A -> A -> Prop) (l : list A) (h : A) (t : list A),
+    Sorted R l -> Sorted R (h :: t) ->
+    (forall x : A, In x l -> R x h) ->
+      Sorted R (l ++ h :: t).
 Proof.
   induction l as [| h t]; simpl; intros.
     assumption.
@@ -69,21 +102,21 @@ Proof.
 Qed.
 
 Lemma Sorted_app :
-  forall (A : LinDec) (l1 l2 : list A),
-    Sorted A l1 -> Sorted A l2 ->
-      (forall x y : A, In x l1 -> In y l2 -> x ≤ y) ->
-        Sorted A (l1 ++ l2).
+  forall (A : Type) (R : A -> A -> Prop) (l1 l2 : list A),
+    Sorted R l1 -> Sorted R l2 ->
+      (forall x y : A, In x l1 -> In y l2 -> R x y) ->
+        Sorted R (l1 ++ l2).
 Proof.
   destruct l2 as [| h2 t2]; cbn; intros.
     rewrite app_nil_r. assumption.
     apply Sorted_app_all; auto.
 Qed.
 
-Hint Resolve Sorted_head Sorted_tail Sorted_app_all.
+Hint Resolve (*Sorted_head*) Sorted_tail Sorted_app_all.
 
 Lemma Sorted_cons :
-  forall (A : LinDec) (h : A) (t : list A),
-    (forall x : A, In x t -> h ≤ x) -> Sorted A t -> Sorted A (h :: t).
+  forall (A : Type) (R : A -> A -> Prop) (h : A) (t : list A),
+    (forall x : A, In x t -> R h x) -> Sorted R t -> Sorted R (h :: t).
 Proof.
   inversion 2; subst.
     auto.
@@ -94,62 +127,87 @@ Proof.
 Qed.
 
 Lemma Sorted_mid :
-  forall (A : LinDec) (x y : A) (l : list A),
-    Sorted A (x :: y :: l) -> Sorted A (x :: l).
+  forall (A : Type) (R : A -> A -> Prop) (x y : A) (l : list A)
+    (R_trans : forall x y z : A, R x y -> R y z -> R x z),
+      Sorted R (x :: y :: l) -> Sorted R (x :: l).
 Proof.
   destruct l.
     auto.
     intros. constructor.
-      assert (x ≤ y) by (apply Sorted_head in H; auto).
+      assert (R x y) by (apply Sorted_head in H; auto).
         apply Sorted_tail in H.
-        assert (y ≤ c) by (apply Sorted_head in H; auto).
-        eapply leq_trans; eauto.
+        assert (R y a) by (apply Sorted_head in H; auto).
+        eapply R_trans; eauto.
       do 2 eapply Sorted_tail. eassumption.
 Qed.
 
 Lemma Sorted_cons_conv :
-  forall (A : LinDec) (h : A) (t : list A),
-    Sorted A (h :: t) -> forall x : A, In x t -> h ≤ x.
+  forall (A : Type) (R : A -> A -> Prop) (h : A) (t : list A)
+    (R_trans : forall x y z : A, R x y -> R y z -> R x z),
+    Sorted R (h :: t) -> forall x : A, In x t -> R h x.
 Proof.
-  induction t as [| h' t'].
-    inversion 2.
-    intros. inversion H0; subst.
-      apply Sorted_head in H. assumption.
-      apply IHt'.
-        apply Sorted_mid in H. assumption.
-        assumption.
+  induction t as [| h' t']; inv 3.
+    apply Sorted_head with t'. assumption.
+    apply IHt'; try assumption.
+      apply Sorted_mid with h'; assumption.
 Qed.
 
 Lemma Sorted_cons_conv' :
-  forall (A : LinDec) (h : A) (t : list A),
-    Sorted A (h :: t) -> forall x : A, In x (h :: t) -> h ≤ x.
+  forall (A : Type) (R : A -> A -> Prop) (h : A) (t : list A)
+    (R_refl : forall x : A, R x x)
+    (R_trans : forall x y z : A, R x y -> R y z -> R x z),
+      Sorted R (h :: t) -> forall x : A, In x (h :: t) -> R h x.
 Proof.
-  induction t as [| h' t'].
-    inversion 2; subst; dec.
-    do 2 inversion 1; subst.
-      dec.
-      inversion H6; subst.
-        assumption.
-        apply IHt'.
-          eapply Sorted_mid; eauto.
-          right. assumption.
+  induction t as [| h' t']; inv 4.
+    inv H1.
+    inv H1.
+      inv H.
+      apply IHt'; try assumption.
+        apply Sorted_mid with h'; assumption.
+        right. assumption.
 Qed.
 
-(* Moved from TrichQuicksortSpec.v *)
+(** An alternative characterization of Sortedness *)
 
-Lemma Sorted_repeat :
-  forall (A : LinDec) (x : A) (n : nat),
-    Sorted A (repeat x n).
+Fixpoint nth {A : Type} (n : nat) (l : list A) {struct l} : option A :=
+match l, n with
+    | [], _ => None
+    | h :: t, 0 => Some h
+    | _ :: t, S n' => nth n' t
+end.
+
+Definition Sorted' {A : Type} (R : A -> A -> Prop) (l : list A) : Prop :=
+  forall (n1 n2 : nat) (x y : A),
+    nth n1 l = Some x -> nth n2 l = Some y -> n1 <= n2 -> R x y.
+
+Lemma Sorted'_Sorted_aux :
+  forall (A : Type) (R : A -> A -> Prop) (l : list A),
+    Sorted' R l -> Sorted R l.
 Proof.
-  induction n as [| n']; cbn.
-    constructor.
-    destruct n'; cbn; constructor; auto.
+  unfold Sorted'. intros.
+  induction l as [| x [| y l]]; constructor.
+    apply (H 0 1 x y); cbn; auto.
+    apply IHl. intros. apply (H (S n1) (S n2)); cbn in *; auto.
+      apply le_n_S. assumption.
 Qed.
 
-Lemma Sorted_filter_eqb :
-  forall (A : LinDec) (x : A) (l : list A),
-    Sorted A (filter (fun x' : A => x' =? x) l).
+Lemma Sorted_Sorted'_aux :
+  forall
+    (A : Type) (R : A -> A -> Prop) (l : list A)
+    (R_refl : forall x : A, R x x)
+    (R_trans : forall x y z : A, R x y -> R y z -> R x z),
+      Sorted R l -> Sorted' R l.
 Proof.
-  intros. destruct (filter_eqb_repeat A x l) as [n H].
-  rewrite H. apply Sorted_repeat.
+  induction 3; unfold Sorted' in *; cbn in *; intros.
+    inv H.
+    destruct n1, n2; inv H; inv H0.
+    destruct n1 as [| [| n1']], n2 as [| [| n2']]; inv H1; inv H2.
+      apply R_trans with y; auto. apply (IHSorted 0 (S n2')); auto.
+        apply le_0_n.
+      inv H3.
+      apply (IHSorted 0 (S n2') x0 y0); auto. apply le_0_n.
+      inv H3.
+      inv H3. inv H2.
+      apply (IHSorted (S n1') (S n2') x0 y0); auto.
+        apply le_S_n. assumption.
 Qed.
